$$
\frac{d}{dx}(c) = 0
$$

$$
\frac{d}{dx}(x) = 1
$$

$$
\frac{d}{dx}(x^2) = 2 \cdot x
$$

$$
\frac{d}{dx}(x^n) = n \cdot x^{n-1}
$$
$$
\frac{d}{dx}(\sqrt{x}) = \frac{1}{2\sqrt{x}}
$$

$$
\frac{d}{dx}(e^x) = e^x
$$

$$
\frac{d}{dx}(\sin(x)) = \cos(x)
$$

$$
\frac{d}{dx}(\cos(x)) = -\sin(x)
$$
$$
\frac{d}{dx}(\tan(x)) = \frac{1}{cos(x)^{2}}
$$

$$
\frac{d}{dx}(\ln(x)) = \frac{1}{x}
$$
$$
\frac{d}{dx}(\arcsin(x)) = \frac{1}{\sqrt{1 - x^2}}
$$

$$
\frac{d}{dx}(\arccos(x)) = -\frac{1}{\sqrt{1 - x^2}}
$$

$$
\frac{d}{dx}(\arctan(x)) = \frac{1}{1 + x^2}
$$

$$
\frac{d}{dx}(\log_a(x)) = \frac{1}{x \ln(a)}
$$

$$
\frac{d}{dx}(a^x) = a^x \ln(a)
$$

$$
\frac{d}{dx}(\sinh(x)) = \cosh(x)
$$

$$
\frac{d}{dx}(\cosh(x)) = \sinh(x)
$$

$$
\frac{d}{dx}(\tanh(x)) = 1 - \tanh^2(x)
$$

## Differentieringsregneregler
$$
f'(x) = \lim_{h \to 0} \frac{f(x + h) - f(x)}{h}
$$

$$
\frac{d}{dx}[f(x) + g(x)] = \frac{d}{dx}[f(x)] + \frac{d}{dx}[g(x)]
$$
## Produktregel:
$$
\frac{d}{dx}[f(x) \cdot g(x)] = \frac{d}{dx}[f(x)] \cdot g(x) + f(x) \cdot \frac{d}{dx}[g(x)]
$$

## KÃ¦deregel:
$$
\frac{d}{dx}[f(g(x))] = f'(g(x)) \cdot g'(x)
$$

$$
\frac{d}{dx} \left[\frac{f(x)}{g(x)}\right] = \frac{f'(x) \cdot g(x) - f(x) \cdot g'(x)}{g(x)^2}
$$