$$\text{Definitioner af hyperbolske funktioner:}$$

$$\sinh(x) = \frac{e^x - e^{-x}}{2}$$
$$\cosh(x) = \frac{e^x + e^{-x}}{2}$$
$$\tanh(x) = \frac{\sinh(x)}{\cosh(x)} = \frac{e^x - e^{-x}}{e^x + e^{-x}}$$
$$\coth(x) = \frac{\cosh(x)}{\sinh(x)} = \frac{e^x + e^{-x}}{e^x - e^{-x}}, \, x \neq 0$$
$$\text{sech}(x) = \frac{1}{\cosh(x)} = \frac{2}{e^x + e^{-x}}$$
$$\text{csch}(x) = \frac{1}{\sinh(x)} = \frac{2}{e^x - e^{-x}}, \, x \neq 0$$

$$\text{Derivater af hyperbolske funktioner:}$$

$$\frac{d}{dx} \sinh(x) = \cosh(x)$$
$$\frac{d}{dx} \cosh(x) = \sinh(x)$$
$$\frac{d}{dx} \tanh(x) = \text{sech}^2(x)$$
$$\frac{d}{dx} \coth(x) = -\text{csch}^2(x)$$
$$\frac{d}{dx} \text{sech}(x) = -\text{sech}(x) \tanh(x)$$
$$\frac{d}{dx} \text{csch}(x) = -\text{csch}(x) \coth(x)$$
