## Opgave 11.1.17 Find the Fourier series of the given function $f(x)$, which is assumed to have the period $2\pi$. Show the details of your work. Sketch or graph the partial sums up to that including $\cos(5x)$ and $\sin(5x)$
Find the Fourier series of the given function $f(x)$, which is
assumed to have the period $2\pi$. Show the details of your
work. Sketch or graph the partial sums up to that including $\cos(5x)$ and $\sin(5x)$

The function is given by:
$$
\quad f(x) =
\begin{cases}
x + \pi, & -\pi \leq x < 0, \\
\pi - x, & 0 \leq x \leq \pi.
\end{cases}
$$

Fourier Series Representation:
$$
f(x) = \frac{a_0}{2} + \sum_{n=1}^{\infty} a_n \cos(nx) + \sum_{n=1}^{\infty} b_n \sin(nx).
$$

$a_{0}$:
$$
a_0 = \frac{1}{\pi} \int_{-\pi}^{\pi} f(x) \, dx.
$$

Splitting into two integrals:
$$
a_0 = \frac{1}{\pi} \left( \int_{-\pi}^{0} (x + \pi) \, dx + \int_{0}^{\pi} (\pi - x) \, dx \right).
$$

Computing each integral separately:
$$
\int_{-\pi}^{0} (x + \pi) \, dx = \int_{-\pi}^{0} x \, dx + \int_{-\pi}^{0} \pi \, dx.
$$
$$
= \left[ \frac{x^2}{2} \right]_{-\pi}^{0} + \pi \left[ x \right]_{-\pi}^{0}
= \left(0 - \frac{\pi^2}{2} \right) + \pi (0 + \pi)
= -\frac{\pi^2}{2} + \pi^2 = \frac{\pi^2}{2}.
$$

For the second integral:
$$
\int_{0}^{\pi} (\pi - x) \, dx = \int_{0}^{\pi} \pi \, dx - \int_{0}^{\pi} x \, dx.
$$
$$
= \pi \left[ x \right]_{0}^{\pi} - \left[ \frac{x^2}{2} \right]_{0}^{\pi}
= \pi^2 - \frac{\pi^2}{2} = \frac{\pi^2}{2}.
$$

$$
a_0 = \frac{1}{\pi} \left( \frac{\pi^2}{2} + \frac{\pi^2}{2} \right) = \frac{\pi^2}{\pi} = \pi.
$$

$a_{n}$:
$$
a_n = \frac{1}{\pi} \int_{-\pi}^{\pi} f(x) \cos(nx) \, dx.
$$

Splitting as before:
$$
a_n = \frac{1}{\pi} \left( \int_{-\pi}^{0} (x + \pi) \cos(nx) \, dx + \int_{0}^{\pi} (\pi - x) \cos(nx) \, dx \right).
$$

Since $f(x)$ is an odd function around $(x=0)$, its cosine coefficients vanish:
$$
a_n = 0, \quad \forall n.
$$

$b_{n}$:
$$
b_n = \frac{1}{\pi} \int_{-\pi}^{\pi} f(x) \sin(nx) \, dx.
$$

Splitting the integral:
$$
b_n = \frac{1}{\pi} \left( \int_{-\pi}^{0} (x + \pi) \sin(nx) \, dx + \int_{0}^{\pi} (\pi - x) \sin(nx) \, dx \right).
$$

Computing separately:

For ($x+\pi$):
$$
\int (x + \pi) \sin(nx) \, dx = \int x \sin(nx) \, dx + \pi \int \sin(nx) \, dx.
$$

Using integration by parts:
$$
\int x \sin(nx) \, dx = -\frac{x}{n} \cos(nx) + \frac{1}{n} \int \cos(nx) \, dx.
$$
$$
= -\frac{x}{n} \cos(nx) + \frac{1}{n^2} \sin(nx).
$$

Evaluating over $[-\pi;0]$ and $[0;\pi]$:
$$
b_n = \frac{2}{n} (1 - (-1)^n).
$$

Thus, the Fourier series expansion is:
$$
f(x) = \frac{\pi}{2} + \sum_{n=1}^{\infty} \frac{2}{n} (1 - (-1)^n) \sin(nx).
$$
Graph:
![[Mat 3 02 lektier.pdf]]

## Fourier coefficients:
![[Mat 3 11.2 FourierrÃ¦kker.png]]
## Simplifications: Even and odd functions
![[Even and odd functions.png]]
## Opgave 11.2.13 Is the given function even or odd or neither even nor odd? Find its Fourier series. Show details of your work.
Is the given function even or odd or neither even nor odd? Find its Fourier series. Show details of your work.
![[11.2.13.png]]

The function $f(x)$ is given as:

$$
f(x) =
\begin{cases}
0, & -\frac{1}{2} \leq x < 0, \\
x, & 0 \leq x \leq \frac{1}{2}.
\end{cases}
$$

I assume the function is extended periodically with period $( T = 1 )$:

$$
f(x + 1) = f(x), \quad \forall x.
$$

A function is **even** if:

$$
f(-x) = f(x).
$$

A function is **odd** if:

$$
f(-x) = -f(x).
$$

I check keypoints:

- For  x in $[0, 1/2]$, $f(x)=x$
- For x in $[-1/2, 0]$, $f(x)=0$

$f(-x)$:

- For x in $[0, 1/2]$, -x in $[-1/2, 0]$, so $f(-x) = 0$
- For x in $[-1/2, 0]$, -x in $[0, 1/2]$, so $f(-x) = -(-x) = x$.

Thus,

$$
f(-x) \neq f(x) \quad \text{(not even)}
$$

$$
f(-x) \neq -f(x) \quad \text{(not odd)}
$$

Since neither condition is satisfied, the function is neither even nor odd.

Fourier Series Representation

The Fourier series of a function with period (1) is:

$$
f(x) = \frac{a_0}{2} + \sum_{n=1}^{\infty} a_n \cos(2\pi n x) + \sum_{n=1}^{\infty} b_n \sin(2\pi n x),
$$

where the coefficients are:

$$
a_0 = \int_{-1/2}^{1/2} f(x) \,dx.
$$

$$
a_n = 2 \int_{-1/2}^{1/2} f(x) \cos(2\pi n x) \,dx.
$$

$$
b_n = 2 \int_{-1/2}^{1/2} f(x) \sin(2\pi n x) \,dx.
$$

Since f(x) = 0 for  $-1/2 \leq x < 0$, the integrals simplify to evaluating only over $[0,1/2]$

$a_{0}$:

$$
a_0 = \int_{-1/2}^{1/2} f(x) \,dx = \int_{0}^{1/2} x \,dx.
$$

$$
a_0 = \left[ \frac{x^2}{2} \right]_{0}^{1/2} = \frac{(1/2)^2}{2} - 0 = \frac{1}{8}.
$$

Thus,

$$
\frac{a_0}{2} = \frac{1}{16}.
$$

$a_{n}$:

$$
a_n = 2 \int_{0}^{1/2} x \cos(2\pi n x) \,dx.
$$

Using integration by parts, let:

- u = x, so du = dx.
- $dv = \cos(2\pi n x) dx$, so $v = \frac{\sin(2\pi n x)}{2\pi n}$

Applying integration by parts:

$$
\int x \cos(2\pi n x) dx = \frac{x \sin(2\pi n x)}{2\pi n} - \int \frac{\sin(2\pi n x)}{2\pi n} dx.
$$

$$
= \frac{x \sin(2\pi n x)}{2\pi n} + \frac{\cos(2\pi n x)}{(2\pi n)^2}.
$$

Evaluating from 0 to $\frac{1}{2}$:

$$
a_n = 2 \left[ \frac{x \sin(2\pi n x)}{2\pi n} + \frac{\cos(2\pi n x)}{(2\pi n)^2} \right]_{0}^{1/2}.
$$

$$
a_n = 2 \left( \frac{(1/2) \sin(\pi n)}{2\pi n} + \frac{\cos(\pi n)}{(2\pi n)^2} - 0 \right).
$$

Since $\sin(\pi n) = 0$, the first term vanishes, leaving:

$$
a_n = 2 \cdot \frac{\cos(\pi n)}{(4\pi^2 n^2)}.
$$

$$
a_n = \frac{\cos(\pi n)}{2\pi^2 n^2}.
$$

$b_{n}$:

$$
b_n = 2 \int_{0}^{1/2} x \sin(2\pi n x) \,dx.
$$

Using integration by parts:

$$
\int x \sin(2\pi n x) dx = -\frac{x \cos(2\pi n x)}{2\pi n} + \int \frac{\cos(2\pi n x)}{2\pi n} dx.
$$

$$
= -\frac{x \cos(2\pi n x)}{2\pi n} + \frac{\sin(2\pi n x)}{(2\pi n)^2}.
$$

Evaluating from 0 to $\frac{1}{2}$:

$$
b_n = 2 \left( -\frac{(1/2) \cos(\pi n)}{2\pi n} + \frac{\sin(\pi n)}{(2\pi n)^2} - 0 \right).
$$

Since $\sin(\pi n) = 0$, the second term vanishes, leaving:

$$
b_n = -2 \cdot \frac{\cos(\pi n)}{4\pi n}.
$$

$$
b_n = -\frac{\cos(\pi n)}{2\pi n}.
$$

Final Fourier Series:
$$
f(x) = \frac{1}{16} + \sum_{n=1}^{\infty} \frac{\cos(\pi n)}{2\pi^2 n^2} \cos(2\pi n x) - \sum_{n=1}^{\infty} \frac{\cos(\pi n)}{2\pi n} \sin(2\pi n x).
$$


## Opgave 11.2.29 Find (a) the Fourier cosine series, (b) the Fourier sine series. Sketch f(x) and its two periodic extensions. Show the details.
Find (a) the Fourier cosine series, (b) the Fourier sine series. Sketch f(x) and its two periodic extensions. Show the details.

$f(x)=\sin(x), \quad (0<x<\pi)$

(a) Fourier Cosine Series:

To find the Fourier cosine series, we extend f(x) **evenly** over $(-\pi, \pi)$, meaning:

$$
f(-x) = f(x).
$$

The Fourier cosine series is:

$$
f(x) = \frac{a_0}{2} + \sum_{n=1}^{\infty} a_n \cos(n x),
$$

where the coefficients are:

$$
a_0 = \frac{2}{\pi} \int_0^{\pi} \sin (x) \,dx.
$$

$$
a_n = \frac{2}{\pi} \int_0^{\pi} \sin (x) \cos(n x) \,dx.
$$

$a_{0}$:

$$
a_0 = \frac{2}{\pi} \int_0^{\pi} \sin (x) \,dx.
$$

$$
= \frac{2}{\pi} [-\cos (x)]_0^{\pi}.
$$

$$
= \frac{2}{\pi} (-\cos (\pi) + \cos (0)).
$$

$$
= \frac{2}{\pi} (-(-1) + 1) = \frac{4}{\pi}.
$$

Thus,

$$
\frac{a_0}{2} = \frac{2}{\pi}.
$$

$a_{n}$:

Using the identity:

$$
\sin (x) \cos(n x) = \frac{1}{2} [\sin(x - n x) + \sin(x + n x)],
$$

we integrate:

$$
a_n = \frac{2}{\pi} \int_0^{\pi} \sin (x) \cos(n x) \,dx.
$$

Using integration by parts or trigonometric identities, we get:

$$
a_n = \frac{2}{\pi} \cdot \frac{(-1)^n - 1}{1 - n^2}, \quad n \neq 1.
$$

For $n = 1$:

$$
a_1 = \frac{2}{\pi} \int_0^{\pi} \sin (x) \cos (x) \,dx = \frac{2}{\pi} \cdot \frac{1}{2} = \frac{1}{\pi}.
$$

Thus, the **Fourier cosine series** is:

$$
f(x) = \frac{2}{\pi} + \sum_{n=1}^{\infty} \frac{2}{\pi} \cdot \frac{(-1)^n - 1}{1 - n^2} \cos(n x).
$$

(b) Fourier Sine Series

To find the Fourier sine series, we extend $f(x)$ **oddly** over $(-\pi, \pi)$, meaning:

$$
f(-x) = -f(x).
$$

The Fourier sine series is:

$$
f(x) = \sum_{n=1}^{\infty} b_n \sin(n x),
$$

where:

$$
b_n = \frac{2}{\pi} \int_0^{\pi} \sin x \sin(n x) \,dx.
$$

$b_{n}$:

Using:

$$
\int_0^{\pi} \sin x \sin(n x) \,dx =
\begin{cases}
\frac{\pi}{2}, & n = 1, \\
0, & n \neq 1.
\end{cases}
$$

So,

$$
b_1 = \frac{2}{\pi} \cdot \frac{\pi}{2} = 1, \quad b_n = 0 \text{ for } n \neq 1.
$$

Thus, the **Fourier sine series** is simply:

$$
f(x) = \sin x.
$$
![[Mat 3 02 lektier.pdf#page=2]]
## Forced oscillations:
$$
my''+cy'+ky=r(t)
$$
where $y=y(t)$ is the displacement from rest, $c$ the damping constant, $k$ the spring constant (spring modulus), and $r(t)$ the external force depending on time $t$. 

### Opgave 11.3.13
Find the steady-state oscillations of $y'' + cy' + y = r(t)$ with $c > 0$ and $r(t)$ as given. Note that the spring constant is $k=1$. Show the details.
$$r(t) = \sum_{n=1}^{N} \left( a_n \cos(n t) + b_n \sin(n t) \right).$$

Solve for the Steady-State Response:

Since the equation is linear and the forcing function is a sum of sines and cosines, we find the steady-state solution by considering a single term at a time:

$$
y_n'' + c y_n' + y_n = a_n \cos(n t) + b_n \sin(n t).
$$

We seek a particular solution of the form:

$$
y_n = A_n \cos(n t) + B_n \sin(n t).
$$

First and second derivatives:
$$
y_n' = -A_n n \sin(n t) + B_n n \cos(n t),
$$

$$
y_n'' = -A_n n^2 \cos(n t) - B_n n^2 \sin(n t).
$$

Substituting into the differential equation:

$$
(-A_n n^2 \cos(n t) - B_n n^2 \sin(n t)) + c (-A_n n \sin(n t) + B_n n \cos(n t)) + (A_n \cos(n t) + B_n \sin(n t)) = a_n \cos(n t) + b_n \sin(n t).
$$

Grouping terms:

$$
(A_n (1 - n^2) + B_n c n) \cos(n t) + (B_n (1 - n^2) - A_n c n) \sin(n t) = a_n \cos(n t) + b_n \sin(n t).
$$

Equating coefficients:

1. For $\cos(n t)$:
   $$
   A_n (1 - n^2) + B_n c n = a_n.
   $$

2. For $\sin(n t)$:
   $$
   B_n (1 - n^2) - A_n c n = b_n.
   $$

---

Solve for $A_{n}$ and $B_{n}$

Rearrange as a system:
$$
\begin{align*}
A_n (1 - n^2) + B_n c n = a_n, \\
B_n (1 - n^2) - A_n c n = b_n.
\end{align*}
$$
Solve for $A_{n}$ and $B_{n}$:

$$A_n = \frac{a_n (1 - n^2) - b_n c n}{(1 - n^2)^2 + c^2 n^2}$$

$$B_n = \frac{b_n (1 - n^2) + a_n c n}{(1 - n^2)^2 + c^2 n^2}$$
General Steady-State Solution:
Summing over all $n$, the steady-state oscillations are:

$$
y_{\text{ss}}(t) = \sum_{n=1}^{N} \left( A_n \cos(n t) + B_n \sin(n t) \right),
$$

where:

$$
A_n = \frac{a_n (1 - n^2) - b_n c n}{(1 - n^2)^2 + c^2 n^2}, \quad
B_n = \frac{b_n (1 - n^2) + a_n c n}{(1 - n^2)^2 + c^2 n^2}.
$$

This provides the steady-state response of the system to the given periodic forcing function.
