![[Pasted image 20250916141434.png]]
$$
F_{net} -F_{f} = \ddot{p}m
$$

Se matlab.

![[Pasted image 20250916150237.png]]
$$
\begin{align*}
m \ddot{p} &=  f_{net}\\
f_{net} &= \underbrace{-kp}_{\text{fjeder}} \, \underbrace{- b \dot{p}}_{\text{d√¶mper}} + F\\
m \ddot{p} &= - kp - b \dot{p} + F\\
\ddot{p} &= \frac{- kp - b \dot{p} + F}{m}\\
\end{align*}
$$
![[Pasted image 20250916152710.png]]
![[Pasted image 20250916152725.png]]
$$
\begin{align*}
m_{2}\ddot{p}_{2} &= f_{\text{net},2}\\
f_{\text{net}, 2} &= F - k(p_{2} - p_{1}) - b(\dot{p}_{2} - \dot{p}_{1})\\
m_{2} \ddot{p}_{2} &= F - k(p_{2} - p_{1}) - b (\dot{p}_{2} - \dot{p}_{1})
\end{align*}
$$